src/program_proof/examples/single_inode_proof.v
@@ -1,6 +1,5 @@
 From RecordUpdate Require Import RecordSet.
 
-From Perennial.algebra Require Import deletable_heap.
 From Perennial.goose_lang Require Import crash_modality.
 From Perennial.program_logic Require Import atomic.
 
