src/program_proof/examples/toy_proof.v
@@ -2,7 +2,6 @@ From RecordUpdate Require Import RecordSet.
 
 From Perennial.Helpers Require Import ModArith.
 From Perennial.goose_lang Require Import crash_modality wpr_lifting.
-From Perennial.algebra Require Import deletable_heap.
 
 From Goose.github_com.mit_pdos.perennial_examples Require Import toy.
 From Perennial.program_logic Require Import na_crash_inv.
